templates/flows/gmap_more.v
@@ -2,334 +2,54 @@ From stdpp Require Export gmap pmap.
 From Coq Require Import PArith.
 Require Import Coq.Setoids.Setoid.
 
-(** Extend stdpp's gmap with a merge function where the merge operation also depends on the key and not just the merged values. *)
+(** Extend stdpp's gmap with a merge function where the merge operation 
+  also depends on the key and not just the merged values. *)
 
-Fixpoint Poimap_raw {A B} (f : positive → A → option B) (t : Pmap_raw A) : Pmap_raw B :=
-  match t with
-  | PLeaf => PLeaf
-  | PNode o l r => PNode' (o ≫= f xH) (Poimap_raw (f ∘ xO) l) (Poimap_raw (f ∘ xI) r)
-  end.
+Definition gmap_imerge `{Countable K} {A B C} 
+  (f : K → option A → option B → option C) 
+  (m1: gmap K A) (m2: gmap K B) : gmap K C :=
+  let fx := λ (k: K) res, match f k (m1 !! k) (m2 !! k) with
+                          | Some x => <[k := x]> res
+                          | None => res end in
+    set_fold fx (∅: gmap K C) (dom m1 ∪ dom m2).
 
-Lemma f_odd: forall A (i: positive) (f: positive -> A), f (i~1%positive) = (f ∘ xI) i.
+Lemma gmap_imerge_lookup_aux `{Countable K} {A B C} 
+    (f : K → option A → option B → option C)
+    (m1 : gmap K A) (m2 : gmap K B) i `{∀ i, f i None None = None} :
+    (i ∈ (dom m1 ∪ dom m2) → gmap_imerge f m1 m2 !! i = f i (m1 !! i) (m2 !! i))
+    ∧ (i ∉ (dom m1 ∪ dom m2) → gmap_imerge f m1 m2 !! i = None).
 Proof.
-  intros.
-  unfold compose.
-  reflexivity.
+  set (P := λ (m': gmap K C) (X: gset K),
+              ∀ x, (x ∈ X → m' !! x = f x (m1 !! x) (m2 !! x))
+                  ∧ (x ∉ X → m' !! x = None) ).
+  apply (set_fold_ind_L P); try done.
+  intros k X res Hk. unfold P. intros HP. intros x.
+  rewrite elem_of_union. rewrite elem_of_singleton. split.
+  - intros [-> | Hx].
+    + destruct (f k (m1 !! k) (m2 !! k)) as [r |] eqn: Hr.
+      by rewrite lookup_insert. by apply HP.
+    + assert (x ≠ k) by set_solver.
+      destruct (f k (m1 !! k) (m2 !! k)) as [r |] eqn: Hr.
+      rewrite lookup_insert_ne; try done. by apply HP.
+      by apply HP in Hx.
+  - intros H'. assert (x ∉ X ∧ x ≠ k) as [Hx Hxk] by set_solver.
+    destruct (f k (m1 !! k) (m2 !! k)) as [r |] eqn: Hr.
+    rewrite lookup_insert_ne; try done. by apply HP.
+    by apply HP in Hx.
 Qed.
 
-Lemma f_even: forall A (i: positive) (f: positive -> A), f (i~0%positive) = (f ∘ xO) i.
-Proof.
-  intros.
-  unfold compose.
-  reflexivity.
-Qed.
-
-Lemma Poimap_wf {A B} (f : positive → A → option B) t : Pmap_wf t → Pmap_wf (Poimap_raw f t).
-Proof. revert f. induction t.
-       - simpl. eauto.
-       - simpl. eauto.
-         intro.
-         intro.
-         unfold PNode'.
-         assert (Pmap_wf t2).
-         unfold Pmap_wf in H.
-         { destruct o.
-           + unfold andb in H.
-             destruct (_ A t2).
-             auto.
-             destruct (_ A t1).
-             contradiction.
-             contradiction.
-           + destruct t2.
-             auto.
-             destruct t1.
-             unfold andb in H at 1.
-             apply H.
-             destruct (match o0 with | Some _ => _ | None => _ end).
-             simpl in H.
-             apply H.
-             simpl in H.
-             contradiction.
-         }
-         assert (Pmap_wf t1).
-         unfold Pmap_wf in H.
-         destruct o.
-         + unfold andb in H.
-           destruct (_ A t1).
-           auto.
-           contradiction.
-         + destruct t1.
-           destruct t2.
-           contradiction.
-           auto.
-           destruct (_ A t2).
-           simpl in H.
-           unfold Pmap_wf.
-           unfold andb in H at 1.
-           destruct (match o with | Some _ => _ | None => _ end).
-           auto.
-           contradiction.
-           unfold andb in H at 1.
-           destruct (match o with | Some _ => _ | None => _ end).
-           contradiction.
-           contradiction.
-         + assert (Pmap_wf (Poimap_raw (f ∘ xO) t1)).
-           apply IHt1.
-           apply H1.
-           assert (Pmap_wf (Poimap_raw (f ∘ xI) t2)).
-           apply IHt2.
-           apply H0.
-           { destruct (Poimap_raw (f ∘ xO) t1).
-             - destruct (o ≫= f 1%positive).
-               unfold Pmap_wf.
-               apply IHt2.
-               apply H0.
-               destruct (Poimap_raw (f ∘ xI) t2).
-               auto.
-               simpl.
-               apply H3.
-             - unfold Pmap_wf.
-               simpl.
-               destruct (o ≫= f 1%positive).
-               unfold andb.
-               unfold Pmap_wf in H2.
-               destruct (match o0 with | Some _ => _ | None => _ end).
-               apply H3.
-               contradiction.
-               unfold andb.
-               unfold Pmap_wf in H2.
-               unfold Pmap_wf in H2.
-               destruct (match o0 with | Some _ => _ | None => _ end).
-               apply H3.
-               contradiction.
-           }
-Qed.
-
-Lemma Poimap_lookup {A B} (f : positive → A → option B) t i :
-  Poimap_raw f t !! i = t !! i ≫= f i.
-Proof.
-  revert f. revert i. induction t as [|o l IHl r IHr]; intros [i|i|]; simpl.
-    + reflexivity.
-    + reflexivity.
-    + reflexivity.
-    + intro. rewrite ?PNode_lookup. simpl.
-      assert (f (i~1%positive) = (f ∘ xI) i).
-      unfold compose.
-      reflexivity.
-      rewrite H. auto.
-    + intro. rewrite ?PNode_lookup. simpl.
-      assert (f (i~0%positive) = (f ∘ xO) i).
-      unfold compose.
-      reflexivity.
-      rewrite H. auto.
-    + intro. rewrite ?PNode_lookup. simpl. auto.
-Qed.
-
-Fixpoint Pimerge_raw {A B C} (f : positive → option A → option B → option C)
-           (t1 : Pmap_raw A) (t2 : Pmap_raw B) : Pmap_raw C :=
-  match t1, t2 with
-  | PLeaf, t2 => Poimap_raw (λ i, f i None ∘ Some) t2
-  | t1, PLeaf => Poimap_raw (λ i, flip (f i) None ∘ Some) t1
-  | PNode o1 l1 r1, PNode o2 l2 r2 =>
-    PNode' (f xH o1 o2) (Pimerge_raw (f ∘ xO) l1 l2) (Pimerge_raw (f ∘ xI) r1 r2)
-  end.
-
-
-Lemma Pimerge_wf {A B C} (f : positive → option A → option B → option C) t1 t2 :
-  Pmap_wf t1 → Pmap_wf t2 → Pmap_wf (Pimerge_raw f t1 t2).
-Proof.
-  revert f. revert t2. induction t1.
-  - intros.
-    apply Poimap_wf. auto.
-  - intros.
-    eauto.
-    simpl.
-    assert (Pmap_wf t1_1).
-    revert H.
-    apply Pmap_wf_l.
-    assert (Pmap_wf t1_2).
-    revert H.
-    apply Pmap_wf_r.
-    unfold Pmap_wf in H.
-    destruct t2;
-      unfold PNode'.
-    assert (Pmap_wf (Poimap_raw ((λ i : positive, flip (f i) None ∘ Some) ∘ xO)
-                                t1_1)).
-    apply Poimap_wf.
-    auto.
-    assert (Pmap_wf (Poimap_raw ((λ i : positive, flip (f i) None ∘ Some) ∘ xI)
-                                t1_2)).
-    apply Poimap_wf.
-    auto.
-
-    +  destruct (Poimap_raw ((λ i : positive, flip (f i) None ∘ Some) ∘ xO)
-                            t1_1).
-       destruct (o ≫= flip (f 1%positive) None ∘ Some);
-         unfold Pmap_wf.
-       rewrite ?andb_True.
-       eauto using Poimap_wf.
-       destruct (Poimap_raw ((λ i : positive, flip (f i) None ∘ Some) ∘ xI)
-                            t1_2).
-       auto.
-       rewrite ?andb_True.
-       auto.
-       eauto using Poimap_wf.
-       unfold Pmap_wf.
-       destruct (o ≫= flip (f 1%positive) None ∘ Some);
-         unfold Pmap_wf.
-       rewrite ?andb_True.
-       eauto.
-       rewrite ?andb_True.
-       eauto.
-    + assert (Pmap_wf  (Pimerge_raw (f ∘ xO) t1_1 t2_1)).
-      apply IHt1_1.
-      auto.
-      revert H0.
-      apply Pmap_wf_l.
-      destruct (Pimerge_raw (f ∘ xO) t1_1 t2_1).
-      destruct (f 1%positive o o0).
-      unfold Pmap_wf.
-      rewrite ?andb_True.
-      split.
-      trivial.
-      apply IHt1_2.
-      auto.
-      revert H0.
-      apply Pmap_wf_r.
-      assert (Pmap_wf  (Pimerge_raw (f ∘ xI) t1_2 t2_2)).
-      apply IHt1_2.
-      auto.
-      revert H0.
-      apply Pmap_wf_r.
-      unfold Pmap_wf.
-      destruct (Pimerge_raw (f ∘ xI) t1_2 t2_2).
-      trivial.
-      rewrite ?andb_True.
-      split.
-      trivial.
-      apply H4.
-      assert (Pmap_wf  (Pimerge_raw (f ∘ xI) t1_2 t2_2)).
-      apply IHt1_2.
-      auto.
-      revert H0.
-      apply Pmap_wf_r.
-      destruct (Pimerge_raw (f ∘ xI) t1_2 t2_2).
-      unfold Pmap_wf.
-      destruct (f 1%positive o o0).
-      rewrite ?andb_True.
-      auto.
-      rewrite ?andb_True.
-      auto.
-      unfold Pmap_wf.
-      destruct (f 1%positive o o0).
-      rewrite ?andb_True.
-      split.
-      apply H3.
-      apply H4.
-      rewrite ?andb_True.
-      split.
-      apply H3.
-      apply H4.
-Qed.
-
-Lemma Pimerge_lookup {A B C} (f : positive → option A → option B → option C)
-    (Hf : ∀ i, f i None None = None) t1 t2 i :
-  Pimerge_raw f t1 t2 !! i = f i (t1 !! i) (t2 !! i).
-Proof.
-  revert Hf. revert f t2 i. induction t1 as [|o1 l1 IHl1 r1 IHr1]; intros f t2 i Hf; unfold Pimerge_raw. simpl.
-  { rewrite Poimap_lookup. by destruct (t2 !! i). }
-  unfold flip.
-  destruct t2 as [|l2 o2 r2]. rewrite Poimap_lookup.
-  destruct (PNode o1 l1 r1 !! i); simpl.
-  - unfold lookup, Plookup_raw. reflexivity.
-  - unfold lookup, Plookup_raw. rewrite Hf. reflexivity.
-  - destruct i; rewrite PNode_lookup; unfold lookup, Plookup_raw.
-    * rewrite f_odd.
-      apply IHr1.
-      intro. unfold compose. apply Hf.
-    * rewrite f_even.
-      apply IHl1.
-      intro. unfold compose. apply Hf.
-    * auto.
-Qed.
-
-Arguments PMap {_} _ _ : assert.
-
-Class Imerge (M : Type → Type) K `{Countable K, (∀ (T: Type), Lookup K T (M T))} :=
-  IMerge
-  {
-    imerge {A B C} (f : K → option A → option B → option C) (m1 : M A) (m2 : M B) : M C;
-    imerge_prf {A B C} (f : K → option A → option B → option C) (m1 : M A) (m2 : M B) (i : K):
-      (∀ j, f j None None = None) -> imerge f m1 m2 !! i = f i (m1 !! i) (m2 !! i)
-  }.
-
-Definition Pimerge {A B C} (f : positive -> option A -> option B -> option C)
-           (m1 : Pmap A) (m2 : Pmap B) :=
-  let (t1,Ht1) := m1 in let (t2,Ht2) := m2 in PMap _ (Pimerge_wf f _ _ Ht1 Ht2).
-
-Lemma Pimerge_prf {A B C} (f : positive → option A → option B → option C)
-    (m1 : Pmap A) (m2 : Pmap B) i (Hf : ∀ i, f i None None = None) :
-    Pimerge f m1 m2 !! i = f i (m1 !! i) (m2 !! i).
-Proof.
-  destruct m1.
-  destruct m2.
-  apply Pimerge_lookup.
-  apply Hf.
-Qed.
-
-Global Instance pmap_positive_imerge : Imerge Pmap positive :=
-  {|
-    imerge A B C := Pimerge;
-    imerge_prf A B C := Pimerge_prf
-  |}.
-
-Lemma gmap_imerge_wf `{Countable K} {A B C}
-    (f : K → option A → option B → option C) m1 m2 :
-  let f' i o1 o2 := match o1, o2 with
-                    | None, None => None
-                    | _, _ =>
-                      decode i ≫= (λ k, f k o1 o2) end
-  in
-  gmap_wf K m1 → gmap_wf K m2 → gmap_wf K (imerge f' m1 m2).
-Proof.
-  intros f'; unfold gmap_wf; rewrite !bool_decide_spec.
-  intros Hm1 Hm2 p z. unfold imerge; simpl.
-  rewrite Pimerge_prf by done; intros.
-  destruct (m1 !! _) eqn:?, (m2 !! _) eqn:?; naive_solver.
-Qed.
-
-Definition gmap_imerge `{Countable K} {A B C}
-           (f : K -> option A -> option B -> option C) (m1 : gmap K A) (m2 : gmap K B)
-           : gmap K C :=
-  let (m1,Hm1) := m1 in
-  let (m2,Hm2) := m2 in
-  let f' i o1 o2 := match o1, o2 with
-                    | None, None => None
-                    | _, _ =>
-                      decode i ≫= (λ k, f k o1 o2)
-                    end
-  in
-  GMap (imerge f' m1 m2) (gmap_imerge_wf f m1 m2 Hm1 Hm2).
-
-Lemma gmap_imerge_prf `{Countable K} {A B C} (f : K → option A → option B → option C)
+Lemma gmap_imerge_lookup `{Countable K} {A B C} 
+    (f : K → option A → option B → option C)
     (m1 : gmap K A) (m2 : gmap K B) i `{∀ i, f i None None = None} :
     gmap_imerge f m1 m2 !! i = f i (m1 !! i) (m2 !! i).
 Proof.
-  destruct m1 as [p1 ?], m2 as [p2 ?].
-  unfold gmap_imerge.
-  unfold lookup; simpl.
-  rewrite Pimerge_prf.
-  case (p1 !! encode i).
-  all: try rewrite decode_encode; auto.
-  case (p2 !! encode i).
-  all: auto.
+  destruct (decide (i ∈ dom m1 ∪ dom m2)) as [Hi | Hi].
+  - apply gmap_imerge_lookup_aux; try done.
+  - assert (i ∉ dom m1 ∧ i ∉ dom m2) as [Hi1 Hi2] by set_solver.
+    apply not_elem_of_dom in Hi1. apply not_elem_of_dom in Hi2.
+    rewrite Hi1. rewrite Hi2. rewrite H0. 
+    apply gmap_imerge_lookup_aux; try done.
 Qed.
-
-Global Instance gmap_Imerge `{Countable K} : Imerge (gmap K) K :=
-  {|
-    imerge A B C := gmap_imerge;
-    imerge_prf A B C := gmap_imerge_prf
-  |}.
 
 Lemma gmap_imerge_empty {A} `{Countable K}
       (f : K → option A → option A → option A)
@@ -338,18 +58,9 @@ Proof.
   intros Hf m.
   rewrite map_eq_iff.
   intros i.
-  rewrite gmap_imerge_prf.
+  rewrite gmap_imerge_lookup.
   replace (empty !! i) with (None : option A).
   all: auto.
-Qed.
-
-Lemma map_Forall_True {A} `{Countable K} (m : gmap K A) (p : K -> A -> Prop) :
-      (∀ (k : K) (a : A), p k a) → (map_Forall p m).
-Proof.
-  intros.
-  unfold map_Forall.
-  intros.
-  apply H0.
 Qed.
 
 
